Homework 08 not completed.

sf/Assignment08_05.v
@@ -7,7 +7,13 @@ Require Export Assignment08_04.
     same as pushing the value of the expression on the stack. *)
 
 Fixpoint s_compile (e : aexp) : list sinstr :=
-  FILL_IN_HERE.
+  match e with
+  | ANum n => [SPush n]
+  | AId id => [SLoad id]
+  | APlus e1 e2 => (s_compile e1) ++ (s_compile e2) ++ [SPlus]
+  | AMinus e1 e2 => (s_compile e1) ++ (s_compile e2) ++ [SMinus]
+  | AMult e1 e2 => (s_compile e1) ++ (s_compile e2) ++ [SMult]
+  end.
 
 (** After you've defined [s_compile], prove the following to test
     that it works. *)
@@ -16,7 +22,7 @@ Example s_compile1 :
     s_compile (AMinus (AId X) (AMult (ANum 2) (AId Y)))
   = [SLoad X; SPush 2; SLoad Y; SMult; SMinus].
 Proof.
-  exact FILL_IN_HERE.
+  reflexivity.
 Qed.
 
 (** **** Exercise: 3 stars, advanced (stack_compiler_correct)  *)
@@ -33,10 +39,37 @@ Qed.
     general lemma to get a usable induction hypothesis; the main
     theorem will then be a simple corollary of this lemma. *)
 
+Lemma s_compile_sub1 : forall st p1 p2 stack,
+  s_execute st stack (p1 ++ p2) = s_execute st (s_execute st stack p1) p2.
+Proof.
+  intros st p1.
+  induction p1.
+  intros.
+  simpl.
+  reflexivity.
+  intros.
+  simpl.
+  destruct stack; destruct a; try (apply IHp1);
+  destruct stack; try (apply IHp1).
+Qed.
+  
+
+Lemma s_compile_sub0 : forall (e : aexp) (st : state) (stack: list nat),
+  s_execute st stack (s_compile e) = aeval st e :: stack.
+Proof.
+  intros e st.
+  induction e; try (intros; simpl; reflexivity);
+  try (simpl; intros; rewrite s_compile_sub1; rewrite s_compile_sub1;
+  rewrite IHe1; rewrite IHe2; reflexivity).
+Qed.
+
+
 Theorem s_compile_correct : forall (st : state) (e : aexp),
   s_execute st [] (s_compile e) = [ aeval st e ].
 Proof.
-  exact FILL_IN_HERE.
+  intros.
+  rewrite s_compile_sub0.
+  reflexivity.
 Qed.
 
 (*-- Check --*)
