sf/Assignment08_04.v
@@ -13,8 +13,49 @@ Theorem no_whiles_terminate: forall c st
     (NOWHL: no_whiles c = true),
   exists st', c / st || st'.
 Proof.
-  exact FILL_IN_HERE.
+  intros.
+  generalize dependent st.
+  induction c.
+  intros.
+  exists st.
+  constructor.
+  intros.
+  exists (update st i (aeval st a)).
+  constructor.
+  reflexivity.
+  intros.
+  inversion NOWHL.
+  apply andb_true_iff in H0.
+  inversion H0.
+  apply IHc1 with (st := st) in H.
+  inversion H.
+  apply IHc2 with (st := x) in H1.
+  inversion H1.
+  exists x0.
+  apply E_Seq with x.
+  apply H2.
+  apply H3.
+  intros.
+  inversion NOWHL.
+  apply andb_true_iff in H0.
+  inversion H0.
+  apply IHc1 with (st := st) in H.
+  inversion H.
+  apply IHc2 with (st := st) in H1.
+  inversion H1.
+  destruct (beval st b) eqn:myH.
+  exists x.
+  apply E_IfTrue.
+  apply myH.
+  apply H2.
+  exists x0.
+  apply E_IfFalse.
+  apply myH.
+  apply H3.
+  intros.
+  inversion NOWHL.
 Qed.
+
 
 (*-- Check --*)
 Check no_whiles_terminate: forall c st
