sf/Assignment08_08.v
@@ -11,8 +11,50 @@ Theorem swap_if_branches: forall b e1 e2,
     (IFB b THEN e1 ELSE e2 FI)
     (IFB BNot b THEN e2 ELSE e1 FI).
 Proof.
-  exact FILL_IN_HERE.
+  unfold cequiv.
+  intros.
+  split.
+  intros.
+  inversion H.
+  subst.
+  apply E_IfFalse.
+  simpl.
+  rewrite H5.
+  reflexivity.
+  apply H6.
+  subst.
+  apply E_IfTrue.
+  simpl.
+  rewrite H5.
+  reflexivity.
+  apply H6.
+  intros.
+  inversion H.
+  subst.
+  apply E_IfFalse.
+  simpl in H5.
+  assert (forall (bo: bool), negb bo = true -> bo = false).
+  intros.
+  destruct bo.
+  inversion H0.
+  reflexivity.
+  apply H0 in H5.
+  apply H5.
+  apply H6.
+  subst.
+  apply E_IfTrue.
+  simpl in H5.
+  assert (forall (bo: bool), negb bo = false -> bo = true).
+  intros.
+  destruct bo.
+  inversion H0.
+  reflexivity.
+  inversion H0.
+  apply H0 in H5.
+  apply H5.
+  apply H6.
 Qed.
+
 
 (*-- Check --*)
 Check swap_if_branches: forall b e1 e2,
