sf/Assignment08_12.v
@@ -7,7 +7,26 @@ Theorem CSeq_congruence : forall c1 c1' c2 c2',
   cequiv c1 c1' -> cequiv c2 c2' ->
   cequiv (c1;;c2) (c1';;c2').
 Proof. 
-  exact FILL_IN_HERE.
+  unfold cequiv.
+  intros.
+  split.
+  intros.
+  inversion H1.
+  subst.
+  apply E_Seq with (st' := st'0).
+  apply H in H4.
+  apply H0 in H7.
+  apply H4.
+  apply H0 in H7.
+  apply H7.
+  intros.
+  inversion H1.
+  subst.
+  apply E_Seq with (st' := st'0).
+  apply H in H4.
+  apply H4.
+  apply H0 in H7.
+  apply H7.
 Qed.
 
 (*-- Check --*)
