sf/Assignment08_13.v
@@ -7,7 +7,38 @@ Theorem CIf_congruence : forall b b' c1 c1' c2 c2',
   bequiv b b' -> cequiv c1 c1' -> cequiv c2 c2' ->
   cequiv (IFB b THEN c1 ELSE c2 FI) (IFB b' THEN c1' ELSE c2' FI).
 Proof.
-  exact FILL_IN_HERE.
+  unfold bequiv; unfold cequiv; simpl.
+  intros.
+  split.
+  intros.
+  inversion H2.
+  subst.
+  apply E_IfTrue.
+  rewrite H in H8.
+  apply H8.
+  apply H0 in H9.
+  apply H9.
+  subst.
+  apply E_IfFalse.
+  rewrite H in H8.
+  apply H8.
+  apply H1 in H9.
+  apply H9.
+  intros.
+  inversion H2.
+  subst.
+  apply E_IfTrue.
+  rewrite <- H in H8.
+  apply H8.
+  apply H0 in H9.
+  apply H9.
+  apply E_IfFalse.
+  subst.
+  rewrite <- H in H8.
+  apply H8.
+  subst.
+  apply H1 in H9.
+  apply H9.
 Qed.
 
 (*-- Check --*)
