sf/Assignment08_16.v
@@ -2,10 +2,21 @@ Require Export Assignment08_15.
 
 (* problem #16: 10 points *)
 
+Lemma APlus_congruence : forall a1 a1' a2 a2',
+  aequiv a1 a1' ->
+  aequiv a2 a2' ->
+  aequiv (APlus a1 a2) (APlus a1' a2').
+Proof.
+  intros. unfold aequiv in *. intros.
+  simpl. auto.
+Qed.
+
 Lemma optimize_0plus_aexp_sound:
   atrans_sound optimize_0plus_aexp.
 Proof.
-  exact FILL_IN_HERE.
+  intros a st.
+  aexp_cases (induction a) Case; simpl;
+  try reflexivity; try (rewrite IHa1; rewrite IHa2; reflexivity).
 Qed.
 
 (*-- Check --*)
