sf/Imp.v
@@ -526,14 +526,37 @@ Proof.
     as elegant as possible. *)
 
 Fixpoint optimize_0plus_b (b : bexp) : bexp :=
-  (* FILL IN HERE *) admit.
+    match b with
+  | BTrue => BTrue
+  | BFalse => BFalse
+  | BEq a1 a2 => BEq (optimize_0plus a1) (optimize_0plus a2)
+  | BLe a1 a2 => BLe (optimize_0plus a1) (optimize_0plus a2)
+  | BNot b1 => BNot (optimize_0plus_b b1)
+  | BAnd b1 b2 => BAnd (optimize_0plus_b b1) (optimize_0plus_b b2)
+  end.
 
 
 Theorem optimize_0plus_b_sound : forall b,
   beval (optimize_0plus_b b) = beval b.
 Proof.
-  (* FILL IN HERE *) Admitted.
-(** [] *)
+  intros.
+  induction b;
+  try (simpl; reflexivity).
+  simpl.
+  rewrite 2 optimize_0plus_sound.
+  reflexivity.
+  simpl.
+  rewrite 2 optimize_0plus_sound.
+  reflexivity.
+  simpl.
+  rewrite IHb.
+  reflexivity.
+  simpl.
+  rewrite IHb1; rewrite IHb2.
+  reflexivity.
+Qed.
+  
+
 
 (** **** Exercise: 4 stars, optional (optimizer)  *)
 (** _Design exercise_: The optimization implemented by our
@@ -953,9 +976,13 @@ Proof.
 Lemma neq_id : forall (T:Type) x y (p q:T), x <> y -> 
                (if eq_id_dec x y then p else q) = q. 
 Proof.
-  (* FILL IN HERE *) Admitted.
-(** [] *)
-
+  intros.
+  unfold not in H.
+  destruct (eq_id_dec x y).
+  apply H in e.
+  inversion e.
+  reflexivity.
+Qed.
 
 End Id. 
 
@@ -989,16 +1016,24 @@ Definition update (st : state) (x : id) (n : nat) : state :=
 Theorem update_eq : forall n x st,
   (update st x n) x = n.
 Proof.
-  (* FILL IN HERE *) Admitted.
-(** [] *)
+  intros.
+  unfold update.
+  rewrite eq_id.
+  reflexivity.
+Qed.
 
 (** **** Exercise: 1 star (update_neq)  *)
 Theorem update_neq : forall x2 x1 n st,
   x2 <> x1 ->                        
   (update st x2 n) x1 = (st x1).
 Proof.
-  (* FILL IN HERE *) Admitted.
-(** [] *)
+  unfold update; unfold not.
+  intros.
+  destruct (eq_id_dec x2 x1).
+  apply H in e.
+  inversion e.
+  reflexivity.
+Qed.
 
 (** **** Exercise: 1 star (update_example)  *)
 (** Before starting to play with tactics, make sure you understand
@@ -1007,31 +1042,55 @@ Proof.
 Theorem update_example : forall (n:nat),
   (update empty_state (Id 2) n) (Id 3) = 0.
 Proof.
-  (* FILL IN HERE *) Admitted.
-(** [] *)
+  intros.
+  reflexivity.
+Qed.
+
 
 (** **** Exercise: 1 star (update_shadow)  *)
 Theorem update_shadow : forall n1 n2 x1 x2 (st : state),
    (update  (update st x2 n1) x2 n2) x1 = (update st x2 n2) x1.
 Proof.
-  (* FILL IN HERE *) Admitted.
-(** [] *)
+  unfold update.
+  intros.
+  destruct (eq_id_dec x2 x1).
+  reflexivity.
+  reflexivity.
+Qed.
+
 
 (** **** Exercise: 2 stars (update_same)  *)
 Theorem update_same : forall n1 x1 x2 (st : state),
   st x1 = n1 ->
   (update st x1 n1) x2 = st x2.
 Proof.
-  (* FILL IN HERE *) Admitted.
-(** [] *)
+  unfold update.
+  intros.
+  destruct (eq_id_dec x1 x2).
+  subst.
+  reflexivity.
+  reflexivity.
+Qed.
+
 
 (** **** Exercise: 3 stars (update_permute)  *)
 Theorem update_permute : forall n1 n2 x1 x2 x3 st,
   x2 <> x1 -> 
   (update (update st x2 n1) x1 n2) x3 = (update (update st x1 n2) x2 n1) x3.
 Proof.
-  (* FILL IN HERE *) Admitted.
-(** [] *)
+  unfold update.
+  intros.
+  destruct (eq_id_dec x1 x3).
+  destruct (eq_id_dec x2 x3).
+  subst.
+  assert (x3 = x3).
+  reflexivity.
+  apply H in H0.
+  inversion H0.
+  reflexivity.
+  reflexivity.
+Qed.
+
 
 (* ################################################### *)
 (** ** Syntax  *)
@@ -1411,8 +1470,15 @@ Example ceval_example2:
     (X ::= ANum 0;; Y ::= ANum 1;; Z ::= ANum 2) / empty_state ||
     (update (update (update empty_state X 0) Y 1) Z 2).
 Proof.
-  (* FILL IN HERE *) Admitted.
-(** [] *)
+  apply E_Seq with (update empty_state X 0).
+  apply E_Ass.
+  reflexivity.
+  apply E_Seq with (update (update empty_state X 0) Y 1).
+  apply E_Ass.
+  reflexivity.
+  apply E_Ass.
+  reflexivity.
+Qed.
 
 (** **** Exercise: 3 stars, advanced (pup_to_n)  *)
 (** Write an Imp program that sums the numbers from [1] to
@@ -1421,15 +1487,37 @@ Proof.
    (this latter part is trickier than you might expect). *)
 
 Definition pup_to_n : com :=
-  (* FILL IN HERE *) admit.
+  Y ::= ANum 0;;
+  WHILE (BNot (BEq (AId X) (ANum 0))) DO
+    Y ::= APlus (AId Y) (AId X);;
+    X ::= AMinus (AId X) (ANum 1)
+  END.
 
 Theorem pup_to_2_ceval :
   pup_to_n / (update empty_state X 2) ||
     update (update (update (update (update (update empty_state
       X 2) Y 0) Y 2) X 1) Y 3) X 0.
 Proof.
-  (* FILL IN HERE *) Admitted.
-(** [] *)
+  apply E_Seq with (update (update empty_state X 2) Y 0).
+  apply E_Ass.
+  reflexivity.
+  apply E_WhileLoop with (update (update (update (update empty_state X 2) Y 0) Y 2) X 1).
+  reflexivity.
+  apply E_Seq with (update (update (update empty_state X 2) Y 0) Y 2).
+  apply E_Ass.
+  reflexivity.
+  apply E_Ass.
+  reflexivity.
+  apply E_WhileLoop with (update (update (update (update (update (update empty_state X 2) Y 0) Y 2) X 1) Y 3) X 0).
+  reflexivity.
+  apply E_Seq with (update (update (update (update (update empty_state X 2) Y 0) Y 2) X 1) Y 3).
+  apply E_Ass.
+  reflexivity.
+  apply E_Ass.
+  reflexivity.
+  apply E_WhileEnd.
+  reflexivity.
+Qed.
 
 
 (* ####################################################### *)
@@ -1527,7 +1615,13 @@ Proof.
      [loopdef] terminates.  Most of the cases are immediately
      contradictory (and so can be solved in one step with
      [inversion]). *)
-  (* FILL IN HERE *) Admitted.
+  induction contra; inversion Heqloopdef.
+  rewrite H1 in H.
+  inversion H.
+  apply IHcontra2.
+  apply Heqloopdef.
+Qed.
+
 (** [] *)
 
 (** **** Exercise: 3 stars (no_whilesR)  *)
@@ -1549,16 +1643,106 @@ Fixpoint no_whiles (c : com) : bool :=
     with [no_whiles]. *)
 
 Inductive no_whilesR: com -> Prop :=
- (* FILL IN HERE *)
-  .
+  | no_0 : no_whilesR SKIP
+  | no_1 : forall id e, no_whilesR (CAss id e)
+  | no_2 : forall c1 c2, no_whilesR c1 -> no_whilesR c2 -> no_whilesR (CSeq c1 c2)
+  | no_3 : forall b c1 c2, no_whilesR c1 -> no_whilesR c2 -> no_whilesR (CIf b c1 c2)
+.
+
+Lemma no_whiles_help:
+  forall c1 c2, no_whiles (c1;; c2) = true -> no_whiles c1 = true.
+Proof.
+  intros.
+  inversion H.
+  unfold andb in H1.
+  destruct (no_whiles c1).
+  rewrite H1.
+  reflexivity.
+  inversion H1.
+Qed.
+
+Lemma no_whiles_help2:
+  forall c1 c2, no_whiles (c1;; c2) = true -> no_whiles c2 = true.
+Proof.
+  intros.
+  inversion H.
+  unfold andb in H1.
+  destruct (no_whiles c1).
+  rewrite H1.
+  reflexivity.
+  inversion H1.
+Qed.
+
 
 Theorem no_whiles_eqv:
    forall c, no_whiles c = true <-> no_whilesR c.
 Proof.
-  (* FILL IN HERE *) Admitted.
-(** [] *)
+  induction c;
+  try (split; intros; constructor; intros; reflexivity).
+  split.
+  intros.
+  constructor.
+  inversion IHc1.
+  apply H0.
+  apply no_whiles_help in H.
+  apply H.
+  apply no_whiles_help2 in H.
+  inversion IHc2.
+  apply H0 in H.
+  apply H.
+  intros.
+  simpl.
+  inversion H.
+  inversion IHc1.
+  inversion IHc2.
+  apply H5 in H2.
+  apply H7 in H3.
+  rewrite H2; rewrite H3.
+  reflexivity.
+  simpl.
+  split.
+  intros.
+  constructor.
+  inversion IHc1.
+  assert (true = no_whiles c1 && no_whiles c2).
+  rewrite H.
+  reflexivity.
+  apply andb_true_eq in H2.
+  inversion H2.
+  assert (no_whiles c1 = true).
+  rewrite H3.
+  reflexivity.
+  apply H0 in H5.
+  apply H5.
+  inversion IHc2.
+  apply H0.
+  assert (true = no_whiles c1 && no_whiles c2).
+  rewrite H.
+  reflexivity.
+  apply andb_true_eq in H2.
+  inversion H2.
+  rewrite H4.
+  reflexivity.
+  intros.
+  inversion IHc1.
+  inversion IHc2.
+  inversion H.
+  apply H1 in H6.
+  apply H3 in H8.
+  rewrite H6.
+  rewrite H8.
+  reflexivity.
+  simpl.
+  split.
+  intros.
+  inversion H.
+  intros.
+  inversion H.
+Qed.
+
 
 (** **** Exercise: 4 stars (no_whiles_terminating)  *)
+
 (** Imp programs that don't involve while loops always terminate.
     State and prove a theorem [no_whiles_terminating] that says this. *)
 (** (Use either [no_whiles] or [no_whilesR], as you prefer.) *)
@@ -1629,27 +1813,57 @@ Inductive sinstr : Type :=
 Fixpoint s_execute (st : state) (stack : list nat)
                    (prog : list sinstr)
                  : list nat :=
-(* FILL IN HERE *) admit.
+let nstack :=
+  match prog with
+  | [] => stack
+  | (SPush n) :: _ => n::stack
+  | (SLoad id) :: _ => (st id)::stack
+  | SPlus::_ => match stack with
+                | n::(m::rest) => (m+n)::rest
+                | _ => stack
+                end
+  | SMinus::_ => match stack with
+                 | n::(m::rest) => (m-n)::rest
+                 | _ => stack
+                 end
+  | SMult::_ => match stack with
+                | n::(m::rest) => (m*n)::rest
+                | _ => stack
+                end
+  end in
+  match prog with
+  | [] => stack
+  | instr::rest => s_execute st nstack rest
+  end
+.
+  
 
 
 Example s_execute1 :
      s_execute empty_state []
        [SPush 5; SPush 3; SPush 1; SMinus]
    = [2; 5].
-(* FILL IN HERE *) Admitted.
+Proof.
+reflexivity. Qed.
 
 Example s_execute2 :
      s_execute (update empty_state X 3) [3;4]
-       [SPush 4; SLoad X; SMult; SPlus]
+    [SPush 4; SLoad X; SMult; SPlus]
    = [15; 4].
-(* FILL IN HERE *) Admitted.
+Proof. reflexivity. Qed.
 
 (** Next, write a function which compiles an [aexp] into a stack
     machine program. The effect of running the program should be the
     same as pushing the value of the expression on the stack. *)
 
 Fixpoint s_compile (e : aexp) : list sinstr :=
-(* FILL IN HERE *) admit.
+  match e with
+  | ANum n => [SPush n]
+  | AId id => [SLoad id]
+  | APlus e1 e2 => (s_compile e1) ++ (s_compile e2) ++ [SPlus]
+  | AMinus e1 e2 => (s_compile e1) ++ (s_compile e2) ++ [SMinus]
+  | AMult e1 e2 => (s_compile e1) ++ (s_compile e2) ++ [SMult]
+  end.
 
 (** After you've defined [s_compile], prove the following to test
     that it works. *)
@@ -1657,8 +1871,7 @@ Fixpoint s_compile (e : aexp) : list sinstr :=
 Example s_compile1 :
     s_compile (AMinus (AId X) (AMult (ANum 2) (AId Y)))
   = [SLoad X; SPush 2; SLoad Y; SMult; SMinus].
-(* FILL IN HERE *) Admitted.
-(** [] *)
+Proof. reflexivity. Qed.
 
 (** **** Exercise: 3 stars, advanced (stack_compiler_correct)  *)
 (** The task of this exercise is to prove the correctness of the
@@ -1674,11 +1887,38 @@ Example s_compile1 :
     general lemma to get a usable induction hypothesis; the main
     theorem will then be a simple corollary of this lemma. *)
 
+Lemma s_compile_sub1 : forall st p1 p2 stack,
+  s_execute st stack (p1 ++ p2) = s_execute st (s_execute st stack p1) p2.
+Proof.
+  intros st p1.
+  induction p1.
+  intros.
+  simpl.
+  reflexivity.
+  intros.
+  apply IHp1.
+Qed.
+  
+
+Lemma s_compile_sub0 : forall (e : aexp) (st : state) (stack: list nat),
+  s_execute st stack (s_compile e) = aeval st e :: stack.
+Proof.
+  intros e st.
+  induction e; try (intros; simpl; reflexivity);
+  try (simpl; intros; rewrite s_compile_sub1; rewrite s_compile_sub1;
+  rewrite IHe1; rewrite IHe2; reflexivity).
+Qed.
+  
+ 
 
 Theorem s_compile_correct : forall (st : state) (e : aexp),
   s_execute st [] (s_compile e) = [ aeval st e ].
 Proof.
-  (* FILL IN HERE *) Admitted.
+  intros.
+  rewrite s_compile_sub0.
+  reflexivity.
+Qed.
+  
 (** [] *)
 
 (** **** Exercise: 5 stars, advanced (break_imp)  *)
